解けたあああああああ！！！！

sort.v
@@ -1,4 +1,4 @@
-Require Import List PeanoNat.
+Require Import List PeanoNat FunInd.
 Import ListNotations.
 From mathcomp Require Import ssreflect.
 
@@ -9,89 +9,70 @@ Module Sort.
 Local Open Scope list_scope.
 Local Open Scope bool_scope.
 
-Lemma length_nil {A: Type}:
-  length ([]: list A) = 0.
-Proof. by []. Qed.
-
-Lemma length_cons {A: Type} (xs: list A) (x: A):
-  length (x :: xs) = S (length xs).
-Proof. by []. Qed.
-
-
-Fixpoint sorted_i (x1: nat) (xs: list nat): bool :=
+Function sorted (xs: list nat): bool :=
   match xs with
   | [] => true
-  | x2 :: xs' => (x1 <=? x2) && sorted_i x2 xs'
+  | x1 :: [] => true
+  | x1 :: (x2 :: _) as xs' => (x1 <=? x2) && sorted xs'
   end.
 
-Definition sorted (xs: list nat): bool :=
-  match xs with
-  | [] => true
-  | x :: [] => true
-  | x :: ys => sorted_i x ys
-  end.
-
-(* x0 :: x1 :: x2 :: x3 :: _*)
-Lemma sorted_i_ind: forall x0 x1 xs,
-  is_true (sorted_i x1 xs) ->
-  x0 <= x1 ->
-  is_true (sorted_i x0 (x1 :: xs)).
+(* (x1 :: x2 :: x3 :: x4 :: _) as xs *)
+Lemma sorted_ind': forall x1 x2 xs3,
+  sorted (x2 :: xs3) = true ->
+  x1 <= x2 ->
+  sorted (x1 :: x2 :: xs3) = true.
 Proof.
-move=> x0 x1 xs Hsorted Hx0_le_x1.
-suff:
-  xs = [] \/ (
-    ( exists x2 xs', xs = x2 :: xs' -> 
-      is_true ( (x1 <=? x2) && sorted_i x1 (x2 :: xs') ) ) ).
-  case => /=.
-  - move=> Hxs.
-    rewrite Hxs /is_true Bool.andb_true_iff Nat.leb_le.
+(*
+induction xsで、
+- xs = []
+- forall xsに対してxs=[x3, xs']
+の2つに分かれてほしい
+*)
+move=> x1 x2 xs3.
+move: x1 x2.
+move: xs3.
+induction xs3.
+- move=> x1 x2 Hsorted Hx1_le_x2.
+  rewrite /sorted Bool.andb_true_iff.
+  split.
+  + by rewrite Nat.leb_le.
+  + by [].
+- move=> x1 x2 Hsorted Hx1_le_x2.
+  rename a into x3.
+  rewrite /sorted.
+  rewrite 2!Bool.andb_true_iff 2!Nat.leb_le.
+  split.
+    by [].
+  split.
+    move: Hsorted.
+    rewrite /sorted.
+    rewrite Bool.andb_true_iff Nat.leb_le.
+    by apply proj1.
+  rewrite -/sorted.
+  suff: sorted xs3 = true.
+    move=> Hxs3_sorted.
+    rewrite Hxs3_sorted.
+    case_eq xs3 => //=.
+    move=> x4 xs4 Hxs4.
+    rewrite Bool.andb_true_iff.
     split.
+    + move: Hsorted.
+      rewrite /sorted Hxs4 2!Bool.andb_true_iff.
+      case. move=> _.
+      case. move=> H _.
       by [].
-      by [].
-  - case.
-    move=> x2.
-    case.
-    move=> xs'.
-    rewrite /is_true 3!Bool.andb_true_iff.
-    split.
-    - by rewrite Nat.leb_le.
-    - move: Hsorted.
-      by rewrite /is_true.
-move: Hsorted.
-rewrite {1}/sorted_i.
-case_eq xs.
-- move=> Hxs _.
-  by left.
-- move=> x2 xs' Hxs.
-  rewrite /is_true Bool.andb_true_iff.
+    + by [].
+  move: Hsorted.
+  rewrite {1}/sorted Bool.andb_true_iff.
   case.
-  move=> Hx1_le_x2.
-  case xs.
+  move=> Hx2_le_x3.
+  rewrite -/sorted. 
+  case_eq xs3.
+    by [].
+  move=> x4 xs4.
+  rewrite Bool.andb_true_iff.
+  move=> _.
+  case.
+  by [].
+Qed.
 
-
-
-
-
-
-
-
-
-Lemma sorted_ind: forall x xs,
-  is_true (sorted xs) -> (forall y, In y xs -> x <= y) -> is_true ( sorted (x :: xs) ).
-Proof.
-move=> x1 xs1 Hsorted Hmin.
-rewrite /is_true /sorted.
-case_eq xs1 => //=.
-move=> x2 xs2 Hxs1.
-case xs2.
-- rewrite Nat.leb_le.
-  specialize (Hmin x2).
-  apply Hmin.
-  rewrite Hxs1.
-  by apply in_eq.
-- move=> x3 xs3.
-Restart.
-move=> x1 xs1 Hsorted Hmin.
-rewrite /is_true /sorted.
-induction xs1.
-by [].
